
# Ejercicios de Alura - Lógica de enunciados: Formalización

El desglose de los ejercicios se realiza por dificultad:

- [🟧 Media](#-media)
- [🟥 Difícil](#-difícil)

## 🟧 Media

>1. $T \rightarrow (W \rightarrow Z)$
>2. $\neg Z \wedge W$
>3. $\therefore \neg T$

<details>
	<summary>Solución</summary>

![](1_medio/01.png)
</details>

<br>
<br>

>1. $Q$
>2. $R \wedge S \rightarrow T$
>3. $P \rightarrow R$
>4. $\therefore Q \rightarrow S$

<details>
	<summary>Solución</summary>

![](1_medio/02.png)
</details>

<br>
<br>

>1. $(A \rightarrow C) \vee (A \rightarrow D)$
>2. $A \rightarrow C \vee D$

<details>
	<summary>Solución</summary>

![](1_medio/03.png)
</details>

<br>
<br>

>1. $P \rightarrow Q$
>2. $T \rightarrow Q \rightarrow W$
>3. $R \rightarrow T$
>4. $\neg (R \rightarrow W)$
>5. $\therefore \neg P$

<details>
	<summary>Solución</summary>

![](1_medio/04.png)
</details>

<br>
<br>

>1. $\neg C$
>2. $\neg D \rightarrow C \wedge K$
>3. $A \rightarrow \neg D$
>4. $\therefore \neg (A \vee C)$

<details>
	<summary>Solución</summary>

![](1_medio/05.png)
</details>

<br>
<br>

>1. $A \rightarrow (B \rightarrow C)$
>2. $\neg B \rightarrow \neg A$
>3. $\therefore A \rightarrow C \vee K$

<details>
	<summary>Solución</summary>

![](1_medio/06.png)
</details>

<br>
<br>

>1. $P \vee (S \rightarrow T)$
>2. $R \wedge S$
>3. $Q \wedge W$
>4. $P \rightarrow T$
>5. $\therefore A \wedge T$

<details>
	<summary>Solución</summary>

![](1_medio/07.png)
</details>

<br>
<br>

>1. $P \rightarrow Q$
>2. $\therefore \neg P \vee Q$

<details>
	<summary>Solución</summary>

![](1_medio/08.png)
</details>

<br>
<br>

>1. $M \vee \neg N \rightarrow \neg P$
>2. $R \rightarrow P$
>3. $R \rightarrow Q$
>4. $\therefore R \rightarrow N \wedge Q$

<details>
	<summary>Solución</summary>

![](1_medio/09.png)
</details>

<br>
<br>

>1. $A \vee B \rightarrow \neg C$
>2. $D \vee K \rightarrow F$
>3. $\neg C \rightarrow \neg F$
>4. $\therefore A \vee B \rightarrow \neg D \wedge \neg K$

<details>
	<summary>Solución</summary>

![](1_medio/10.png)
</details>

<br>
<br>

>1. $P \vee (Q \wedge R)$
>2. $\therefore P \vee Q$

<details>
	<summary>Solución</summary>

![](1_medio/11.png)
</details>

<br>
<br>

>1. $\neg A \vee B$
>2. $\therefore A \rightarrow B$

<details>
	<summary>Solución</summary>

![](1_medio/12.png)
</details>

<br>
<br>

>1. $R \rightarrow B$
>2. $T \rightarrow S$
>3. $T \vee R$
>4. $\therefore S \vee Q$

<details>
	<summary>Solución</summary>

![](1_medio/13.png)
</details>

<br>
<br>

>1. $P \rightarrow Q \vee R$
>2. $Q \rightarrow R$
>3. $R \rightarrow S$
>4. $\therefore P \rightarrow S$

<details>
	<summary>Solución</summary>

![](1_medio/14.png)
</details>

<br>
<br>

>1. $A \rightarrow \neg C$
>2. $B \rightarrow C$
>3. $\therefore \neg (A \wedge B)$

<details>
	<summary>Solución</summary>

![](1_medio/15.png)
</details>

<br>
<br>

>1. $S \vee (R \wedge T)$
>2. $T \wedge Q \rightarrow S$
>3. $T \rightarrow R \wedge Q$
>4. $\therefore S$

<details>
	<summary>Solución</summary>

![](1_medio/16.png)
</details>

<br>
<br>

>1. $\neg R \rightarrow \neg Q \wedge S$
>2. $R \vee \neg Q \rightarrow (S \rightarrow Q)$
>3. $\therefore R$

<details>
	<summary>Solución</summary>

![](1_medio/17.png)
</details>

<br>
<br>

>1. $P \vee Q$
>2. $\neg P$
>3. $\therefore Q$

<details>
	<summary>Solución</summary>

![](1_medio/18.png)
</details>

<br>
<br>

>1. $P \rightarrow Q$
>2. $P \rightarrow \neg Q$
>3. $\therefore \neg P$

<details>
	<summary>Solución</summary>

![](1_medio/19.png)
</details>

<br>
<br>

>1. $\neg (P \rightarrow R)$
>2. $P \rightarrow (Q \rightarrow R)$
>3. $\therefore Q \rightarrow (P \wedge R)$

<details>
	<summary>Solución</summary>

![](1_medio/20.png)
</details>

<br>
<br>

>1. $T \rightarrow (W \rightarrow Z)$
>2. $\neg Z \wedge W$
>3. $\therefore \neg T$

<details>
	<summary>Solución</summary>

![](1_medio/21.png)
</details>

<br>
<br>

>1. $P \rightarrow \neg S$
>2. $D \rightarrow \neg C$
>3. $S \rightarrow C$
>4. $\therefore S \rightarrow \neg D \wedge \neg P$

<details>
	<summary>Solución</summary>

![](1_medio/22.png)
</details>

<br>
<br>

>1. $A \vee B$
>2. $A \rightarrow C$
>3. $\neg D \rightarrow \neg B$
>4. $\therefore C \vee D$

<details>
	<summary>Solución</summary>

![](1_medio/23.png)
</details>

<br>
<br>

>1. $P \vee Q$
>2. $\neg T$
>3. $Q \rightarrow T$
>4. $\therefore \neg (P \vee (R \wedge S))$

<details>
	<summary>Solución</summary>

![](1_medio/24.png)
</details>

<br>
<br>

>1. $G \rightarrow A \vee B$
>2. $A \rightarrow C \vee D$
>3. $B \rightarrow K \wedge F$
>4. $\neg D$
>5. $\therefore G \rightarrow C \vee K$

<details>
	<summary>Solución</summary>

![](1_medio/25.png)
</details>

<br>
<br>

>1. $G \rightarrow A \vee B$
>2. $A \rightarrow C \vee D$
>3. $B \rightarrow K \wedge F$
>4. $\neg D$
>5. $\therefore G \rightarrow C \vee K$

<details>
	<summary>Solución</summary>

![](1_medio/25.png)
</details>

<br>
<br>

>1. $\neg (P \wedge Q)$
>2. $\therefore \neg P \vee \neg Q$

<details>
	<summary>Solución</summary>

![](1_medio/26.png)
</details>

### 🟥 Difícil
